Add some more to soundness

theories/Core/Soundness/LogicalRelation/Definitions.v
@@ -10,14 +10,23 @@ Global Open Scope predicate_scope.
 
 Generalizable All Variables.
 
-Notation "'typ_pred'" := (predicate (Tcons ctx (Tcons typ Tnil))).
-Notation "'typ_pred_equivalence'" := (@predicate_equivalence (Tcons ctx (Tcons typ Tnil))).
-Notation "'glu_pred'" := (predicate (Tcons ctx (Tcons exp (Tcons typ (Tcons domain Tnil))))).
-Notation "'glu_pred_equivalence'" := (@predicate_equivalence (Tcons ctx (Tcons exp (Tcons typ (Tcons domain Tnil))))).
-
+Notation "'glu_typ_pred_args'" := (Tcons ctx (Tcons typ Tnil)).
+Notation "'glu_typ_pred'" := (predicate glu_typ_pred_args).
+Notation "'glu_typ_pred_equivalence'" := (@predicate_equivalence glu_typ_pred_args).
 Notation "Γ ⊢ A ® R" := ((R Γ A : Prop) : Prop) (in custom judg at level 80, Γ custom exp, A custom exp, R constr).
+
+Notation "'glu_exp_pred_args'" := (Tcons ctx (Tcons exp (Tcons typ (Tcons domain Tnil)))).
+Notation "'glu_exp_pred'" := (predicate glu_exp_pred_args).
+Notation "'glu_exp_pred_equivalence'" := (@predicate_equivalence glu_exp_pred_args).
 Notation "Γ ⊢ M : A ® m ∈ R" := (R Γ M A m : (Prop : Type)) (in custom judg at level 80, Γ custom exp, M custom exp, A custom exp, m custom domain, R constr).
+
+Notation "'glu_sub_pred_args'" := (Tcons ctx (Tcons sub (Tcons env Tnil))).
+Notation "'glu_sub_pred'" := (predicate glu_sub_pred_args).
+Notation "'glu_sub_pred_equivalence'" := (@predicate_equivalence glu_sub_pred_args).
+Notation "Γ ⊢s σ ® ρ ∈ R" := (R Γ σ ρ : Prop) (in custom judg at level 80, Γ custom exp, σ custom exp, ρ custom domain, R constr).
+
 Notation "'Glu' a ≈ b ∈ R ↘ P ↘ El" := (R P El a b : Prop) (in custom judg at level 90, a custom domain, b custom domain, R constr, P constr, El constr).
+Notation "'EG' A ∈ R ↘ Sb " := (R Sb A : Prop) (in custom judg at level 90, A custom exp, R constr, Sb constr).
 
 Inductive glu_nat : ctx -> exp -> domain -> Prop :=
 | glu_nat_zero :
@@ -35,33 +44,33 @@ Inductive glu_nat : ctx -> exp -> domain -> Prop :=
 #[export]
 Hint Constructors glu_nat : mcltt.
 
-Definition nat_typ_pred i : typ_pred := fun Γ M => {{ Γ ⊢ M ≈ ℕ : Type@i }}.
-Arguments nat_typ_pred i Γ M/.
+Definition nat_glu_typ_pred i : glu_typ_pred := fun Γ M => {{ Γ ⊢ M ≈ ℕ : Type@i }}.
+Arguments nat_glu_typ_pred i Γ M/.
 
-Definition nat_glu_pred i : glu_pred := fun Γ m M a => {{ Γ ⊢ M ® nat_typ_pred i }} /\ glu_nat Γ m a.
-Arguments nat_glu_pred i Γ m M a/.
+Definition nat_glu_exp_pred i : glu_exp_pred := fun Γ m M a => {{ Γ ⊢ M ® nat_glu_typ_pred i }} /\ glu_nat Γ m a.
+Arguments nat_glu_exp_pred i Γ m M a/.
 
-Definition neut_typ_pred i C : typ_pred :=
+Definition neut_glu_typ_pred i C : glu_typ_pred :=
   fun Γ M => {{ Γ ⊢ M : Type@i }} /\
             (forall Δ σ V, {{ Δ ⊢w σ : Γ }} -> {{ Rne C in length Δ ↘ V }} -> {{ Δ ⊢ M[σ] ≈ V : Type@i }}).
-Arguments neut_typ_pred i C Γ M/.
+Arguments neut_glu_typ_pred i C Γ M/.
 
-Inductive neut_glu_pred i C : glu_pred :=
-| mk_neut_glu_pred : forall Γ m M A c,
-    {{ Γ ⊢ M ® neut_typ_pred i C }} ->
+Inductive neut_glu_exp_pred i C : glu_exp_pred :=
+| mk_neut_glu_exp_pred : forall Γ m M A c,
+    {{ Γ ⊢ M ® neut_glu_typ_pred i C }} ->
     {{ Dom c ≈ c ∈ per_bot }} ->
     (forall Δ σ V v, {{ Δ ⊢w σ : Γ }} ->
                 {{ Rne C in length Δ ↘ V }} ->
                 {{ Rne c in length Δ ↘ v }} ->
                 {{ Δ ⊢ m[σ] ≈ v : M[σ] }}) ->
-    {{ Γ ⊢ m : M ® ⇑ A c ∈ neut_glu_pred i C }}.
+    {{ Γ ⊢ m : M ® ⇑ A c ∈ neut_glu_exp_pred i C }}.
 
-Inductive pi_typ_pred i
+Inductive pi_glu_typ_pred i
   (IR : relation domain)
-  (IP : typ_pred)
-  (IEl : glu_pred)
-  (OP : forall c c' (equiv_c_c' : {{ Dom c ≈ c' ∈ IR }}), typ_pred) : typ_pred :=
-| mk_pi_typ_pred : forall Γ IT OT M,
+  (IP : glu_typ_pred)
+  (IEl : glu_exp_pred)
+  (OP : forall c c' (equiv_c_c' : {{ Dom c ≈ c' ∈ IR }}), glu_typ_pred) : glu_typ_pred :=
+| mk_pi_glu_typ_pred : forall Γ IT OT M,
     {{ Γ ⊢ M ≈ Π IT OT : Type@i }} ->
     {{ Γ , IT ⊢ OT : Type@i }} ->
     (forall Δ σ, {{ Δ ⊢w σ : Γ }} -> {{ Δ ⊢ IT[σ] ® IP }}) ->
@@ -70,15 +79,15 @@ Inductive pi_typ_pred i
         {{ Δ ⊢ m : IT[σ] ® a ∈ IEl }} ->
         forall (equiv_a_a : {{ Dom a ≈ a ∈ IR }}),
           {{ Δ ⊢ OT[σ,,m] ® OP _ _ equiv_a_a }}) ->
-    {{ Γ ⊢ M ® pi_typ_pred i IR IP IEl OP }}.
+    {{ Γ ⊢ M ® pi_glu_typ_pred i IR IP IEl OP }}.
 
-Inductive pi_glu_pred i
+Inductive pi_glu_exp_pred i
   (IR : relation domain)
-  (IP : typ_pred)
-  (IEl : glu_pred)
+  (IP : glu_typ_pred)
+  (IEl : glu_exp_pred)
   (elem_rel : relation domain)
-  (OEl : forall c c' (equiv_c_c' : {{ Dom c ≈ c' ∈ IR }}), glu_pred): glu_pred :=
-| mk_pi_glu_pred : forall Γ IT OT m M a,
+  (OEl : forall c c' (equiv_c_c' : {{ Dom c ≈ c' ∈ IR }}), glu_exp_pred): glu_exp_pred :=
+| mk_pi_glu_exp_pred : forall Γ IT OT m M a,
     {{ Γ ⊢ m : M }} ->
     {{ Dom a ≈ a ∈ elem_rel }} ->
     {{ Γ ⊢ M ≈ Π IT OT : Type@i }} ->
@@ -89,61 +98,49 @@ Inductive pi_glu_pred i
         {{ Δ ⊢ m' : IT[ σ ] ® b ∈ IEl }} ->
         forall (equiv_b_b : {{ Dom b ≈ b ∈ IR }}),
         exists ab, {{ $| a & b |↘ ab }} /\ {{ Δ ⊢ m[σ] m' : OT[σ,,m'] ® ab ∈ OEl _ _ equiv_b_b }}) ->
-    {{ Γ ⊢ m : M ® a ∈ pi_glu_pred i IR IP IEl elem_rel OEl }}.
+    {{ Γ ⊢ m : M ® a ∈ pi_glu_exp_pred i IR IP IEl elem_rel OEl }}.
 
 #[export]
-Hint Constructors neut_glu_pred pi_typ_pred pi_glu_pred : mcltt.
+Hint Constructors neut_glu_exp_pred pi_glu_typ_pred pi_glu_exp_pred : mcltt.
 
-Lemma pi_glu_pred_pi_typ_pred : forall i IR IP IEl (OP : forall c c' (equiv_c_c' : {{ Dom c ≈ c' ∈ IR }}), typ_pred) elem_rel OEl Γ m M a,
-    {{ Γ ⊢ m : M ® a ∈ pi_glu_pred i IR IP IEl elem_rel OEl }} ->
-    (forall Δ m' M' b c c' (equiv_c_c' : {{ Dom c ≈ c' ∈ IR }}),
-        {{ Δ ⊢ m' : M' ® b ∈ OEl _ _ equiv_c_c' }} ->
-        {{ Δ ⊢ M' ® OP _ _ equiv_c_c' }}) ->
-    {{ Γ ⊢ M ® pi_typ_pred i IR IP IEl OP }}.
-Proof.
-  inversion_clear 1; econstructor; eauto.
-  intros.
-  edestruct H5 as [? []]; eauto.
-Qed.
-
-Definition univ_typ_pred j i : typ_pred := fun Γ T => {{ Γ ⊢ T ≈ Type@j :  Type@i }}.
-Arguments univ_typ_pred j i Γ T/.
+Definition univ_glu_typ_pred j i : glu_typ_pred := fun Γ T => {{ Γ ⊢ T ≈ Type@j :  Type@i }}.
+Arguments univ_glu_typ_pred j i Γ T/.
 
 Section Gluing.
   Variable
     (i : nat)
-      (glu_univ_typ_rec : forall {j}, j < i -> domain -> typ_pred).
+      (glu_univ_typ_rec : forall {j}, j < i -> domain -> glu_typ_pred).
 
-  Definition univ_glu_pred' {j} (lt_j_i : j < i) : glu_pred :=
+  Definition univ_glu_exp_pred' {j} (lt_j_i : j < i) : glu_exp_pred :=
     fun Γ m M A =>
       {{ Γ ⊢ m : M }} /\
         {{ Γ ⊢ M ≈ Type@j : Type@i }} /\
         {{ Γ ⊢ m ® glu_univ_typ_rec lt_j_i A }}.
 
   #[global]
-  Arguments univ_glu_pred' {j} lt_j_i Γ m M A/.
+  Arguments univ_glu_exp_pred' {j} lt_j_i Γ m M A/.
 
-  Inductive glu_univ_elem_core : typ_pred -> glu_pred -> domain -> domain -> Prop :=
+  Inductive glu_univ_elem_core : glu_typ_pred -> glu_exp_pred -> domain -> domain -> Prop :=
   | glu_univ_elem_core_univ :
     `{ forall typ_rel
          el_rel
          (lt_j_i : j < i),
           j = j' ->
-          typ_rel <∙> univ_typ_pred j i ->
-          el_rel <∙> univ_glu_pred' lt_j_i ->
+          typ_rel <∙> univ_glu_typ_pred j i ->
+          el_rel <∙> univ_glu_exp_pred' lt_j_i ->
           {{ Glu 𝕌@j ≈ 𝕌@j' ∈ glu_univ_elem_core ↘ typ_rel ↘ el_rel }} }
 
   | glu_univ_elem_core_nat :
     `{ forall typ_rel el_rel,
-          typ_rel <∙> nat_typ_pred i ->
-          el_rel <∙> nat_glu_pred i ->
+          typ_rel <∙> nat_glu_typ_pred i ->
+          el_rel <∙> nat_glu_exp_pred i ->
           {{ Glu ℕ ≈ ℕ ∈ glu_univ_elem_core ↘ typ_rel ↘ el_rel }} }
 
   | glu_univ_elem_core_pi :
     `{ forall (in_rel : relation domain)
          IP IEl
-         (OP : forall c c' (equiv_c_c' : {{ Dom c ≈ c' ∈ in_rel }}), typ_pred)
-         (OEl : forall c c' (equiv_c_c' : {{ Dom c ≈ c' ∈ in_rel }}), glu_pred)
+         (OP : forall c c' (equiv_c_c' : {{ Dom c ≈ c' ∈ in_rel }}), glu_typ_pred)
+         (OEl : forall c c' (equiv_c_c' : {{ Dom c ≈ c' ∈ in_rel }}), glu_exp_pred)
          typ_rel el_rel
          (elem_rel : relation domain),
           {{ Glu a ≈ a' ∈ glu_univ_elem_core ↘ IP ↘ IEl }} ->
@@ -153,57 +150,57 @@ Section Gluing.
               {{ ⟦ B' ⟧ p' ↦ c' ↘ b' }} ->
               {{ Glu b ≈ b' ∈ glu_univ_elem_core ↘ OP _ _ equiv_c_c' ↘ OEl _ _ equiv_c_c' }}) ->
           {{ DF Π a p B ≈ Π a' p' B' ∈ per_univ_elem i ↘ elem_rel }} ->
-          typ_rel <∙> pi_typ_pred i in_rel IP IEl OP ->
-          el_rel <∙> pi_glu_pred i in_rel IP IEl elem_rel OEl ->
+          typ_rel <∙> pi_glu_typ_pred i in_rel IP IEl OP ->
+          el_rel <∙> pi_glu_exp_pred i in_rel IP IEl elem_rel OEl ->
           {{ Glu Π a p B ≈ Π a' p' B' ∈ glu_univ_elem_core ↘ typ_rel ↘ el_rel }} }
 
   | glu_univ_elem_core_neut :
     `{ forall typ_rel el_rel,
           {{ Dom b ≈ b' ∈ per_bot }} ->
-          typ_rel <∙> neut_typ_pred i b ->
-          el_rel <∙> neut_glu_pred i b ->
+          typ_rel <∙> neut_glu_typ_pred i b ->
+          el_rel <∙> neut_glu_exp_pred i b ->
           {{ Glu ⇑ a b ≈ ⇑ a' b' ∈ glu_univ_elem_core ↘ typ_rel ↘ el_rel }} }.
 End Gluing.
 
 #[export]
 Hint Constructors glu_univ_elem_core : mcltt.
 
-Equations glu_univ_elem (i : nat) : typ_pred -> glu_pred -> domain -> domain -> Prop by wf i :=
+Equations glu_univ_elem (i : nat) : glu_typ_pred -> glu_exp_pred -> domain -> domain -> Prop by wf i :=
 | i => glu_univ_elem_core i (fun j lt_j_i A Γ M => exists P El, {{ Glu A ≈ A ∈ glu_univ_elem j ↘ P ↘ El }} /\ {{ Γ ⊢ M ® P }}).
 
-Definition glu_univ (i : nat) (A : domain) (B : domain) : typ_pred :=
+Definition glu_univ_typ (i : nat) (A : domain) (B : domain) : glu_typ_pred :=
   fun Γ M => exists P El, {{ Glu A ≈ B ∈ glu_univ_elem i ↘ P ↘ El }} /\ {{ Γ ⊢ M ® P }}.
-Arguments glu_univ i A B Γ M/.
+Arguments glu_univ_typ i A B Γ M/.
 
-Definition univ_glu_pred j i : glu_pred :=
+Definition univ_glu_pred j i : glu_exp_pred :=
     fun Γ m M A =>
       {{ Γ ⊢ m : M }} /\ {{ Γ ⊢ M ≈ Type@j : Type@i }} /\
-        {{ Γ ⊢ m ® glu_univ j A A }}.
+        {{ Γ ⊢ m ® glu_univ_typ j A A }}.
 Arguments univ_glu_pred j i Γ t T a/.
 
 Section GluingInduction.
   Hypothesis
-    (motive : nat -> typ_pred -> glu_pred -> domain -> domain -> Prop)
+    (motive : nat -> glu_typ_pred -> glu_exp_pred -> domain -> domain -> Prop)
 
       (case_univ :
         forall i (j j' : nat)
-          (typ_rel : typ_pred) (el_rel : glu_pred) (lt_j_i : j < i),
+          (typ_rel : glu_typ_pred) (el_rel : glu_exp_pred) (lt_j_i : j < i),
           j = j' ->
           (forall P El A B, {{ Glu A ≈ B ∈ glu_univ_elem j ↘ P ↘ El }} -> motive j P El A B) ->
-          typ_rel <∙> univ_typ_pred j i ->
+          typ_rel <∙> univ_glu_typ_pred j i ->
           el_rel <∙> univ_glu_pred j i ->
           motive i typ_rel el_rel d{{{ 𝕌 @ j }}} d{{{ 𝕌 @ j' }}})
 
       (case_nat :
-        forall i (typ_rel : typ_pred) (el_rel : glu_pred),
-          typ_rel <∙> nat_typ_pred i ->
-          el_rel <∙> nat_glu_pred i ->
+        forall i (typ_rel : glu_typ_pred) (el_rel : glu_exp_pred),
+          typ_rel <∙> nat_glu_typ_pred i ->
+          el_rel <∙> nat_glu_exp_pred i ->
           motive i typ_rel el_rel d{{{ ℕ }}} d{{{ ℕ }}})
 
       (case_pi :
-        forall i (a a' : domain) (B : typ) (p : env) (B' : typ) (p' : env) (in_rel : relation domain) (IP : typ_pred)
-          (IEl : glu_pred) (OP : forall c c' : domain, {{ Dom c ≈ c' ∈ in_rel }} -> typ_pred)
-          (OEl : forall c c' : domain, {{ Dom c ≈ c' ∈ in_rel }} -> glu_pred) (typ_rel : typ_pred) (el_rel : glu_pred)
+        forall i (a a' : domain) (B : typ) (p : env) (B' : typ) (p' : env) (in_rel : relation domain) (IP : glu_typ_pred)
+          (IEl : glu_exp_pred) (OP : forall c c' : domain, {{ Dom c ≈ c' ∈ in_rel }} -> glu_typ_pred)
+          (OEl : forall c c' : domain, {{ Dom c ≈ c' ∈ in_rel }} -> glu_exp_pred) (typ_rel : glu_typ_pred) (el_rel : glu_exp_pred)
           (elem_rel : relation domain),
           {{ Glu a ≈ a' ∈ glu_univ_elem i ↘ IP ↘ IEl }} ->
           motive i IP IEl a a' ->
@@ -217,17 +214,17 @@ Section GluingInduction.
               {{ ⟦ B' ⟧ p' ↦ c' ↘ b' }} ->
               motive i (OP c c' equiv_c_c') (OEl c c' equiv_c_c') b b') ->
           {{ DF Π a p B ≈ Π a' p' B' ∈ per_univ_elem i ↘ elem_rel }} ->
-          typ_rel <∙> pi_typ_pred i in_rel IP IEl OP ->
-          el_rel <∙> pi_glu_pred i in_rel IP IEl elem_rel OEl ->
+          typ_rel <∙> pi_glu_typ_pred i in_rel IP IEl OP ->
+          el_rel <∙> pi_glu_exp_pred i in_rel IP IEl elem_rel OEl ->
           motive i typ_rel el_rel d{{{ Π a p B }}} d{{{ Π a' p' B' }}})
 
       (case_neut :
         forall i (b b' : domain_ne) (a a' : domain)
-          (typ_rel : typ_pred)
-          (el_rel : glu_pred),
+          (typ_rel : glu_typ_pred)
+          (el_rel : glu_exp_pred),
           {{ Dom b ≈ b' ∈ per_bot }} ->
-          typ_rel <∙> neut_typ_pred i b ->
-          el_rel <∙> neut_glu_pred i b ->
+          typ_rel <∙> neut_glu_typ_pred i b ->
+          el_rel <∙> neut_glu_exp_pred i b ->
           motive i typ_rel el_rel d{{{ ⇑ a b }}} d{{{ ⇑ a' b' }}})
   .
 
@@ -240,7 +237,7 @@ Section GluingInduction.
   | i, P, El, a, b, H =>
       glu_univ_elem_core_ind
         i
-        (fun j lt_j_i A Γ M => glu_univ j A A Γ M)
+        (fun j lt_j_i A Γ M => glu_univ_typ j A A Γ M)
         (motive i)
         (fun j j' typ_rel el_rel lt_j_i Heq Htr Hel =>
            case_univ i j j' typ_rel el_rel lt_j_i
@@ -261,7 +258,7 @@ End GluingInduction.
 Inductive glu_neut i A B Γ m M c : Prop :=
 | mk_glu_neut :
     {{ Γ ⊢ m : M }} ->
-    {{ Γ ⊢ M ® glu_univ i A B }} ->
+    {{ Γ ⊢ M ® glu_univ_typ i A B }} ->
     {{ Dom c ≈ c ∈ per_bot }} ->
     (forall Δ σ a, {{ Δ ⊢w σ : Γ }} -> {{ Rne c in length Δ ↘ a }} -> {{ Δ ⊢ m[σ] ≈ a : M[σ] }}) ->
     {{ Γ ⊢ m : M ® c ∈ glu_neut i A B }}.
@@ -269,7 +266,7 @@ Inductive glu_neut i A B Γ m M c : Prop :=
 Inductive glu_norm i A B Γ m M a : Prop :=
 | mk_glu_norm :
     {{ Γ ⊢ m : M }} ->
-    {{ Γ ⊢ M ® glu_univ i A B }} ->
+    {{ Γ ⊢ M ® glu_univ_typ i A B }} ->
     {{ Dom ⇓ A a ≈ ⇓ B a ∈ per_top }} ->
     (forall Δ σ b, {{ Δ ⊢w σ : Γ }} -> {{ Rnf ⇓ A a in length Δ ↘ b }} -> {{ Δ ⊢ m [ σ ] ≈  b : M [ σ ] }}) ->
     {{ Γ ⊢ m : M ® a ∈ glu_norm i A B }}.
@@ -283,12 +280,94 @@ Inductive glu_typ i A B Γ M : Prop :=
 
 Ltac invert_glu_rel1 :=
   match goal with
-  | H : pi_typ_pred _ _ _ _ _ _ _ |- _ =>
+  | H : pi_glu_typ_pred _ _ _ _ _ _ _ |- _ =>
       progressive_invert H
-  | H : pi_glu_pred _ _ _ _ _ _ _ _ _ _ |- _ =>
+  | H : pi_glu_exp_pred _ _ _ _ _ _ _ _ _ _ |- _ =>
       progressive_invert H
-  | H : neut_typ_pred _ _ _ _ |- _ =>
+  | H : neut_glu_typ_pred _ _ _ _ |- _ =>
       progressive_invert H
-  | H : neut_glu_pred _ _ _ _ _ _ |- _ =>
+  | H : neut_glu_exp_pred _ _ _ _ _ _ |- _ =>
       progressive_invert H
   end.
+
+Variant glu_rel_typ_sub i Δ A σ ρ : Prop :=
+| mk_glu_typ_sub :
+  `{ forall P El,
+        {{ ⟦ A ⟧ ρ ↘ a }} ->
+        {{ Glu a ≈ a ∈ glu_univ_elem i ↘ P ↘ El }} ->
+        {{ Δ ⊢ A[σ] ® P }} ->
+        glu_rel_typ_sub i Δ A σ ρ }.
+
+Definition nil_glu_sub_pred : glu_sub_pred :=
+  fun Δ σ ρ => {{ Δ ⊢s σ : ⋅ }}.
+Arguments nil_glu_sub_pred Δ σ ρ/.
+
+(* The parameters are ordered differently from the Agda version
+   so that we can return "glu_sub_pred". *)
+Variant cons_glu_sub_pred i Γ A (TSb : glu_sub_pred) : glu_sub_pred :=
+| mk_cons_glu_sub_pred :
+  `{ forall P El,
+        {{ Δ ⊢s σ : Γ, A }} ->
+        (* Do we need the following argument?
+           In other words, is it possible to prove that "TSb" respects
+           wf_sub_eq without the following condition? *)
+        {{ Δ ⊢s Wk ∘ σ ≈ Wk∘σ : Γ }} ->
+        {{ ⟦ A ⟧ ρ ↯ ↘ a }} ->
+        {{ Glu a ≈ a ∈ glu_univ_elem i ↘ P ↘ El }} ->
+        {{ Δ ⊢ #0[σ] : A[Wk∘σ] ® ~(ρ 0) ∈ El }} ->
+        {{ Δ ⊢s σ ® ρ ∈ cons_glu_sub_pred i Γ A TSb }} }.
+
+Inductive glu_ctx_env : glu_sub_pred -> ctx -> Prop :=
+| glu_ctx_env_nil :
+  `{ forall Sb,
+        Sb <∙> nil_glu_sub_pred ->
+        {{ EG ⋅ ∈ glu_ctx_env ↘ Sb }} }
+| glu_ctx_env_cons :
+  `{ forall i TSb Sb,
+        {{ EG Γ ∈ glu_ctx_env ↘ TSb }} ->
+        {{ Γ ⊢ A : Type@i }} ->
+        (forall Δ σ ρ,
+            {{ Δ ⊢s σ ® ρ ∈ TSb }} ->
+            glu_rel_typ_sub i Δ A σ ρ) ->
+        Sb <∙> cons_glu_sub_pred i Γ A TSb ->
+        {{ EG Γ, A ∈ glu_ctx_env ↘ Sb }} }.
+
+Variant glu_rel_exp_sub i Δ M A σ ρ : Prop :=
+| mk_glu_exp_sub :
+  `{ forall P El,
+        {{ ⟦ A ⟧ ρ ↘ a }} ->
+        {{ ⟦ M ⟧ ρ ↘ m }} ->
+        {{ Glu a ≈ a ∈ glu_univ_elem i ↘ P ↘ El }} ->
+        {{ Δ ⊢ M[σ] : A[σ] ® m ∈ El }} ->
+        glu_rel_exp_sub i Δ M A σ ρ }.
+
+Variant glu_rel_sub_sub Δ τ (Sb : glu_sub_pred) σ ρ : Prop :=
+| mk_glu_sub_sub :
+  `{ {{ ⟦ τ ⟧s ρ ↘ ρ' }} ->
+     {{ Δ ⊢s τ ∘ σ ® ρ' ∈ Sb }} ->
+     glu_rel_sub_sub Δ τ Sb σ ρ}.
+
+Definition glu_rel_ctx Γ : Prop := exists Sb, {{ EG Γ ∈ glu_ctx_env ↘ Sb }}.
+Arguments glu_rel_ctx Γ/.
+
+Definition glu_rel_exp Γ M A : Prop :=
+  exists Sb,
+    {{ EG Γ ∈ glu_ctx_env ↘ Sb }} /\
+      exists i,
+      forall Δ σ ρ,
+        {{ Δ ⊢s σ ® ρ ∈ Sb }} ->
+        glu_rel_exp_sub i Δ M A σ ρ.
+Arguments glu_rel_exp Γ M A/.
+
+Definition glu_rel_sub Γ τ Γ' : Prop :=
+  exists Sb Sb',
+    {{ EG Γ ∈ glu_ctx_env ↘ Sb }} /\
+    {{ EG Γ' ∈ glu_ctx_env ↘ Sb' }} /\
+      forall Δ σ ρ,
+        {{ Δ ⊢s σ ® ρ ∈ Sb }} ->
+        glu_rel_sub_sub Δ τ Sb' σ ρ.
+Arguments glu_rel_sub Γ τ Γ'/.
+
+Notation "⊩ Γ" := (glu_rel_ctx Γ) (in custom judg at level 80, Γ custom exp).
+Notation "Γ ⊩ M : A" := (glu_rel_exp Γ M A) (in custom judg at level 80, Γ custom exp, M custom exp, A custom exp).
+Notation "Γ ⊩s τ : Γ'" := (glu_rel_sub Γ τ Γ') (in custom judg at level 80, Γ custom exp, τ custom exp, Γ' custom exp).
